Move rejection_sample_coefficient_lemma to Spec.MLDSA.Math.fst

libcrux-ml-dsa/src/simd/portable/sample.rs
@@ -1,39 +1,5 @@
 use crate::constants::FIELD_MODULUS;
 
-#[hax_lib::fstar::before(
-r#"#push-options "--z3rlimit 1500 --max_fuel 3 --max_ifuel 3 --ext context_pruning --z3refresh"
-
-let rejection_sample_coefficient_lemma (randomness:Seq.seq u8) (i:nat{i < (Seq.length randomness) / 3}) :
-  Lemma (let b0 = cast (Seq.index randomness (i * 3)) <: i32 in
-        let b1 = cast (Seq.index randomness (i * 3 + 1)) <: i32 in
-        let b2 = cast (Seq.index randomness (i * 3 + 2)) <: i32 in
-        let coefficient = (((b2 <<! mk_i32 16) |. (b1 <<! mk_i32 8)) |. b0) &.
-            mk_i32 8388607 in
-        Spec.MLDSA.Math.rejection_sample_coefficient randomness i == coefficient) =
-  let b0 = cast (Seq.index randomness (i * 3)) <: i32 in
-  let b1 = cast (Seq.index randomness (i * 3 + 1)) <: i32 in
-  let b2 = cast (Seq.index randomness (i * 3 + 2)) <: i32 in
-  let b2' = if b2 >. mk_i32 127 then b2 -. mk_i32 128  else b2 in
-  assert_norm (pow2 23 == 8388608);
-  assert (b2' == (b2 %! mk_i32 128));
-  assert (((mk_i32 (pow2 16) *. b2) %! mk_i32 (pow2 23)) == (mk_i32 (pow2 16) *. (b2 %! mk_i32 128)));
-  logor_disjoint (b2 <<! mk_i32 16) (b1 <<! mk_i32 8) 16;
-  assert (((b2 <<! mk_i32 16) |. (b1 <<! mk_i32 8)) == ((b2 <<! mk_i32 16) +. (b1 <<! mk_i32 8)));
-  logor_disjoint ((b2 <<! mk_i32 16) |. (b1 <<! mk_i32 8)) b0 8;
-  assert ((((b2 <<! mk_i32 16) |. (b1 <<! mk_i32 8)) |. b0) ==
-    (((b2 <<! mk_i32 16) +. (b1 <<! mk_i32 8)) +. b0));
-  assert ((b2 <<! mk_i32 16) == (mk_i32 (pow2 16) *. b2));
-  assert ((b1 <<! mk_i32 8) == (mk_i32 (pow2 8) *. b1));
-  logand_mask_lemma (((mk_i32 (pow2 16) *. b2) +. (mk_i32 (pow2 8) *. b1)) +. b0) 23;
-  assert (((((mk_i32 (pow2 16) *. b2) +. ((mk_i32 (pow2 8) *. b1)) +. b0)) %! mk_i32 (pow2 23)) ==
-    ((((mk_i32 (pow2 16) *. b2) %! mk_i32 (pow2 23)) +. ((mk_i32 (pow2 8) *. b1)) +. b0)));
-  assert (((((mk_i32 (pow2 16) *. b2) +. (mk_i32 (pow2 8) *. b1)) +. b0) %! mk_i32 (pow2 23)) ==
-    (((mk_i32 (pow2 16) *. (b2 %! mk_i32 128)) +. (mk_i32 (pow2 8) *. b1)) +. b0));
-  assert (((((mk_i32 (pow2 16) *. b2) +. (mk_i32 (pow2 8) *. b1)) +. b0) %! mk_i32 (pow2 23)) ==
-    (((mk_i32 (pow2 16) *. b2') +. (mk_i32 (pow2 8) *. b1)) +. b0))
-
-#pop-options"#
-)]
 #[inline(always)]
 #[hax_lib::requires(fstar!(r#"Seq.length randomness / 3 <= Lib.IntTypes.max_size_t /\
     Seq.length $randomness / 3 <= Seq.length $out"#))]
@@ -64,7 +30,7 @@ pub fn rejection_sample_less_than_field_modulus(randomness: &[u8], out: &mut [i3
 
         let coefficient = ((b2 << 16) | (b1 << 8) | b0) & 0x00_7F_FF_FF;
         hax_lib::fstar!(
-            r#"rejection_sample_coefficient_lemma $randomness (v $i);
+            r#"Spec.MLDSA.Math.rejection_sample_coefficient_lemma $randomness (v $i);
             Lib.LoopCombinators.unfold_repeati (v $i + 1) 
                 (Spec.MLDSA.Math.rejection_sample_field_modulus_inner $randomness) Seq.empty (v $i)"#
         );
