libcrux-ml-dsa/proofs/fstar/extraction/Libcrux_ml_dsa.Simd.Portable.Sample.fst
@@ -3,39 +3,6 @@ module Libcrux_ml_dsa.Simd.Portable.Sample
 open Core
 open FStar.Mul
 
-#push-options "--z3rlimit 1500 --max_fuel 3 --max_ifuel 3 --ext context_pruning --z3refresh"
-
-let rejection_sample_coefficient_lemma (randomness:Seq.seq u8) (i:nat{i < (Seq.length randomness) / 3}) :
-  Lemma (let b0 = cast (Seq.index randomness (i * 3)) <: i32 in
-        let b1 = cast (Seq.index randomness (i * 3 + 1)) <: i32 in
-        let b2 = cast (Seq.index randomness (i * 3 + 2)) <: i32 in
-        let coefficient = (((b2 <<! mk_i32 16) |. (b1 <<! mk_i32 8)) |. b0) &.
-            mk_i32 8388607 in
-        Spec.MLDSA.Math.rejection_sample_coefficient randomness i == coefficient) =
-  let b0 = cast (Seq.index randomness (i * 3)) <: i32 in
-  let b1 = cast (Seq.index randomness (i * 3 + 1)) <: i32 in
-  let b2 = cast (Seq.index randomness (i * 3 + 2)) <: i32 in
-  let b2' = if b2 >. mk_i32 127 then b2 -. mk_i32 128  else b2 in
-  assert_norm (pow2 23 == 8388608);
-  assert (b2' == (b2 %! mk_i32 128));
-  assert (((mk_i32 (pow2 16) *. b2) %! mk_i32 (pow2 23)) == (mk_i32 (pow2 16) *. (b2 %! mk_i32 128)));
-  logor_disjoint (b2 <<! mk_i32 16) (b1 <<! mk_i32 8) 16;
-  assert (((b2 <<! mk_i32 16) |. (b1 <<! mk_i32 8)) == ((b2 <<! mk_i32 16) +. (b1 <<! mk_i32 8)));
-  logor_disjoint ((b2 <<! mk_i32 16) |. (b1 <<! mk_i32 8)) b0 8;
-  assert ((((b2 <<! mk_i32 16) |. (b1 <<! mk_i32 8)) |. b0) ==
-    (((b2 <<! mk_i32 16) +. (b1 <<! mk_i32 8)) +. b0));
-  assert ((b2 <<! mk_i32 16) == (mk_i32 (pow2 16) *. b2));
-  assert ((b1 <<! mk_i32 8) == (mk_i32 (pow2 8) *. b1));
-  logand_mask_lemma (((mk_i32 (pow2 16) *. b2) +. (mk_i32 (pow2 8) *. b1)) +. b0) 23;
-  assert (((((mk_i32 (pow2 16) *. b2) +. ((mk_i32 (pow2 8) *. b1)) +. b0)) %! mk_i32 (pow2 23)) ==
-    ((((mk_i32 (pow2 16) *. b2) %! mk_i32 (pow2 23)) +. ((mk_i32 (pow2 8) *. b1)) +. b0)));
-  assert (((((mk_i32 (pow2 16) *. b2) +. (mk_i32 (pow2 8) *. b1)) +. b0) %! mk_i32 (pow2 23)) ==
-    (((mk_i32 (pow2 16) *. (b2 %! mk_i32 128)) +. (mk_i32 (pow2 8) *. b1)) +. b0));
-  assert (((((mk_i32 (pow2 16) *. b2) +. (mk_i32 (pow2 8) *. b1)) +. b0) %! mk_i32 (pow2 23)) ==
-    (((mk_i32 (pow2 16) *. b2') +. (mk_i32 (pow2 8) *. b1)) +. b0))
-
-#pop-options
-
 let rejection_sample_less_than_field_modulus (randomness: t_Slice u8) (out: t_Slice i32) =
   let sampled:usize = mk_usize 0 in
   let e_out_len:usize = Core.Slice.impl__len #i32 out in
@@ -73,7 +40,7 @@ let rejection_sample_less_than_field_modulus (randomness: t_Slice u8) (out: t_Sl
             mk_i32 8388607
           in
           let _:Prims.unit =
-            rejection_sample_coefficient_lemma randomness (v i);
+            Spec.MLDSA.Math.rejection_sample_coefficient_lemma randomness (v i);
             Lib.LoopCombinators.unfold_repeati (v i + 1)
               (Spec.MLDSA.Math.rejection_sample_field_modulus_inner randomness)
               Seq.empty
