libcrux-ml-dsa/proofs/fstar/spec/Spec.MLDSA.Math.fst
@@ -59,3 +59,36 @@ let rejection_sample_eta_4_inner
 let rejection_sample_eta_4 (randomness:Seq.seq u8) : (Seq.seq i32) =
   Lib.LoopCombinators.repeati (Seq.length randomness)
     (rejection_sample_eta_4_inner randomness) Seq.empty
+
+#push-options "--z3rlimit 1500 --max_fuel 3 --max_ifuel 3 --ext context_pruning --z3refresh"
+
+let rejection_sample_coefficient_lemma (randomness:Seq.seq u8) (i:nat{i < (Seq.length randomness) / 3}) :
+  Lemma (let b0 = cast (Seq.index randomness (i * 3)) <: i32 in
+        let b1 = cast (Seq.index randomness (i * 3 + 1)) <: i32 in
+        let b2 = cast (Seq.index randomness (i * 3 + 2)) <: i32 in
+        let coefficient = (((b2 <<! mk_i32 16) |. (b1 <<! mk_i32 8)) |. b0) &.
+            mk_i32 8388607 in
+        Spec.MLDSA.Math.rejection_sample_coefficient randomness i == coefficient) =
+  let b0 = cast (Seq.index randomness (i * 3)) <: i32 in
+  let b1 = cast (Seq.index randomness (i * 3 + 1)) <: i32 in
+  let b2 = cast (Seq.index randomness (i * 3 + 2)) <: i32 in
+  let b2' = if b2 >. mk_i32 127 then b2 -. mk_i32 128  else b2 in
+  assert_norm (pow2 23 == 8388608);
+  assert (b2' == (b2 %! mk_i32 128));
+  assert (((mk_i32 (pow2 16) *. b2) %! mk_i32 (pow2 23)) == (mk_i32 (pow2 16) *. (b2 %! mk_i32 128)));
+  logor_disjoint (b2 <<! mk_i32 16) (b1 <<! mk_i32 8) 16;
+  assert (((b2 <<! mk_i32 16) |. (b1 <<! mk_i32 8)) == ((b2 <<! mk_i32 16) +. (b1 <<! mk_i32 8)));
+  logor_disjoint ((b2 <<! mk_i32 16) |. (b1 <<! mk_i32 8)) b0 8;
+  assert ((((b2 <<! mk_i32 16) |. (b1 <<! mk_i32 8)) |. b0) ==
+    (((b2 <<! mk_i32 16) +. (b1 <<! mk_i32 8)) +. b0));
+  assert ((b2 <<! mk_i32 16) == (mk_i32 (pow2 16) *. b2));
+  assert ((b1 <<! mk_i32 8) == (mk_i32 (pow2 8) *. b1));
+  logand_mask_lemma (((mk_i32 (pow2 16) *. b2) +. (mk_i32 (pow2 8) *. b1)) +. b0) 23;
+  assert (((((mk_i32 (pow2 16) *. b2) +. ((mk_i32 (pow2 8) *. b1)) +. b0)) %! mk_i32 (pow2 23)) ==
+    ((((mk_i32 (pow2 16) *. b2) %! mk_i32 (pow2 23)) +. ((mk_i32 (pow2 8) *. b1)) +. b0)));
+  assert (((((mk_i32 (pow2 16) *. b2) +. (mk_i32 (pow2 8) *. b1)) +. b0) %! mk_i32 (pow2 23)) ==
+    (((mk_i32 (pow2 16) *. (b2 %! mk_i32 128)) +. (mk_i32 (pow2 8) *. b1)) +. b0));
+  assert (((((mk_i32 (pow2 16) *. b2) +. (mk_i32 (pow2 8) *. b1)) +. b0) %! mk_i32 (pow2 23)) ==
+    (((mk_i32 (pow2 16) *. b2') +. (mk_i32 (pow2 8) *. b1)) +. b0))
+
+#pop-options
